Otway-Rees: renamed some attacker Lemmas with misleading names
Since the Otway-Rees protocol cannot achieve authentication, the Lemma names
were misleading in that they tried to proof that one party believes of the
authentication of the other or that both parties believe in mutual auth.
The wording "believe to talk to" is more appropriate in this context, as it
is decided based on the terms stored in the respective final principal states.

otway-rees/OYRS.Attacker.fst
@@ -286,7 +286,7 @@ let attacker_knows_conv_key_stored_in_initiator_or_responder_state
     if k_ab = conv_key then () else error "attacker could not derive conversation key\n"
   | _ -> error "not a final principal state\n"
 
-val initiator_believes_responder_authenticated:
+val initiator_believes_talking_to_responder:
   i:principal ->
   si:nat ->
   r:principal ->
@@ -294,7 +294,7 @@ val initiator_believes_responder_authenticated:
   (requires (fun t0 -> True))
   (ensures (fun t0 _ t1 -> True))
 
-let initiator_believes_responder_authenticated
+let initiator_believes_talking_to_responder
   i
   si
   r
@@ -305,9 +305,9 @@ let initiator_believes_responder_authenticated
     if b = r then () else error "initiator does not believe to talk to responder\n"
   | _ -> error "wrong state\n"
 
-/// This function can be used to check for mutual authentication between
-/// initiator and responder at runtime
-val initiator_and_responder_mutually_authenticated:
+/// This function can be used to check whether initiator and responder talk to
+/// each other at runtime
+val initiator_and_responder_talk_to_each_other:
   initiator:principal ->
   responder:principal ->
   i_sess_idx:nat ->
@@ -316,7 +316,7 @@ val initiator_and_responder_mutually_authenticated:
   (requires (fun t0 -> True))
   (ensures (fun t0 _ t1 -> True))
 
-let initiator_and_responder_mutually_authenticated
+let initiator_and_responder_talk_to_each_other
   initiator
   responder
   i_sess_idx
@@ -329,7 +329,10 @@ let initiator_and_responder_mutually_authenticated
   | Success (S.InitiatorRecvedMsg4 srv b k_ab) -> (
     match OYRS.Sessions.parse_session_st r_sess with
     | Success (S.ResponderSentMsg4 srv' a k_ab') -> (
-      if a = initiator && b = responder && k_ab = k_ab' then () else error "mutual authentication not achieved\n"
+      if a <> initiator then error "responder does not believe to talk to initiator\n"
+      else if b <> responder then error "initiator does not believe to talk to responder\n"
+      else if k_ab <> k_ab' then error "initiator and responder have different keys\n"
+      else ()
     )
     | _ -> error "wrong initiator final session\n"
   )
